theories/Operational/Common/OSCausalityContract.v
@@ -1,0 +1,348 @@
+From Stdlib Require Import List Arith.PeanoNat Lia.
+Import ListNotations.
+From RocqSched Require Import Foundation.Base.
+From RocqSched Require Import Semantics.Schedule.
+From RocqSched Require Import Multicore.Common.MultiCoreBase.
+From RocqSched Require Import Multicore.Common.Admissibility.
+From RocqSched Require Import Operational.Common.State.
+From RocqSched Require Import Operational.Common.Step.
+From RocqSched Require Import Operational.Common.Invariants.
+From RocqSched Require Import Operational.Common.StepLemmas.
+From RocqSched Require Import Operational.Common.OSProjectionInterface.
+From RocqSched Require Import Operational.Common.ConcreteExecution.
+From RocqSched Require Import Operational.Common.Projection.
+From RocqSched Require Import Operational.Common.OSLocalAdapterContract.
+
+Lemma op_running_job_not_dispatch_pending_in_range :
+  forall m st c_run j c,
+    op_struct_inv m st ->
+    op_current st c_run = Some j ->
+    c < m ->
+    op_dispatch_target st c <> Some j.
+Proof.
+  intros m st c_run j c Hinv Hcur Hlt Hpending.
+  destruct Hinv as [_ _ Hnotin _ Hdispatchrun].
+  pose proof (Hnotin c_run j Hcur) as Hnotrunnable.
+  pose proof (Hdispatchrun c j Hlt Hpending) as Hin.
+  contradiction.
+Qed.
+
+Record labeled_concrete_scheduling_causality_contract
+    {CState : Type}
+    {P : OSLabeledProjection CState}
+    (jobs : JobId -> Job)
+    (m : nat)
+    (ex : labeled_concrete_execution P m) : Prop :=
+  mkLabeledConcreteSchedulingCausalityContract {
+    lcsc_wakeup_released :
+      forall t j,
+        os_step_label P (lce_trace ex t) (lce_trace ex (S t)) = EvWakeup j ->
+        released jobs j (S t);
+    lcsc_wakeup_visible :
+      forall t j,
+        os_step_label P (lce_trace ex t) (lce_trace ex (S t)) = EvWakeup j ->
+        In j
+           (op_runnable
+              (os_to_op_state (osl_to_os_projection P) (lce_trace ex (S t))));
+    lcsc_request_sets_need_resched :
+      forall t c,
+        c < m ->
+        os_step_label P (lce_trace ex t) (lce_trace ex (S t)) = EvRequestResched c ->
+        op_need_resched
+          (os_to_op_state (osl_to_os_projection P) (lce_trace ex (S t)))
+          c = true;
+    lcsc_handle_sets_need_resched :
+      forall t c,
+        c < m ->
+        os_step_label P (lce_trace ex t) (lce_trace ex (S t)) = EvHandleResched c ->
+        op_need_resched
+          (os_to_op_state (osl_to_os_projection P) (lce_trace ex (S t)))
+          c = true;
+    lcsc_choose_sets_dispatch_target :
+      forall t c j,
+        c < m ->
+        os_step_label P (lce_trace ex t) (lce_trace ex (S t)) = EvChoose c j ->
+        op_dispatch_target
+          (os_to_op_state (osl_to_os_projection P) (lce_trace ex (S t)))
+          c = Some j;
+    lcsc_choose_from_runnable :
+      forall t c j,
+        c < m ->
+        os_step_label P (lce_trace ex t) (lce_trace ex (S t)) = EvChoose c j ->
+        In j
+           (op_runnable
+              (os_to_op_state (osl_to_os_projection P) (lce_trace ex t)));
+    lcsc_dispatch_sets_current :
+      forall t c j,
+        c < m ->
+        os_step_label P (lce_trace ex t) (lce_trace ex (S t)) = EvDispatch c j ->
+        op_current
+          (os_to_op_state (osl_to_os_projection P) (lce_trace ex (S t)))
+          c = Some j;
+    lcsc_dispatch_clears_dispatch_target :
+      forall t c j,
+        c < m ->
+        os_step_label P (lce_trace ex t) (lce_trace ex (S t)) = EvDispatch c j ->
+        op_dispatch_target
+          (os_to_op_state (osl_to_os_projection P) (lce_trace ex (S t)))
+          c = None;
+    lcsc_dispatch_clears_need_resched :
+      forall t c j,
+        c < m ->
+        os_step_label P (lce_trace ex t) (lce_trace ex (S t)) = EvDispatch c j ->
+        op_need_resched
+          (os_to_op_state (osl_to_os_projection P) (lce_trace ex (S t)))
+          c = false;
+    lcsc_dispatch_removes_from_runnable :
+      forall t c j,
+        c < m ->
+        os_step_label P (lce_trace ex t) (lce_trace ex (S t)) = EvDispatch c j ->
+        ~ In j
+             (op_runnable
+                (os_to_op_state (osl_to_os_projection P) (lce_trace ex (S t))));
+    lcsc_preempt_sets_current :
+      forall t c old new,
+        c < m ->
+        os_step_label P (lce_trace ex t) (lce_trace ex (S t)) =
+        EvPreempt c old new ->
+        op_current
+          (os_to_op_state (osl_to_os_projection P) (lce_trace ex (S t)))
+          c = Some new;
+    lcsc_preempt_requeues_old :
+      forall t c old new,
+        c < m ->
+        os_step_label P (lce_trace ex t) (lce_trace ex (S t)) =
+        EvPreempt c old new ->
+        In old
+           (op_runnable
+              (os_to_op_state (osl_to_os_projection P) (lce_trace ex (S t))));
+    lcsc_preempt_removes_new_from_runnable :
+      forall t c old new,
+        c < m ->
+        os_step_label P (lce_trace ex t) (lce_trace ex (S t)) =
+        EvPreempt c old new ->
+        ~ In new
+             (op_runnable
+                (os_to_op_state (osl_to_os_projection P) (lce_trace ex (S t))));
+    lcsc_preempt_clears_dispatch_target :
+      forall t c old new,
+        c < m ->
+        os_step_label P (lce_trace ex t) (lce_trace ex (S t)) =
+        EvPreempt c old new ->
+        op_dispatch_target
+          (os_to_op_state (osl_to_os_projection P) (lce_trace ex (S t)))
+          c = None;
+    lcsc_preempt_clears_need_resched :
+      forall t c old new,
+        c < m ->
+        os_step_label P (lce_trace ex t) (lce_trace ex (S t)) =
+        EvPreempt c old new ->
+        op_need_resched
+          (os_to_op_state (osl_to_os_projection P) (lce_trace ex (S t)))
+          c = false;
+    lcsc_complete_sets_completed :
+      forall t j,
+        os_step_label P (lce_trace ex t) (lce_trace ex (S t)) = EvComplete j ->
+        completed
+          jobs
+          m
+          (project_schedule (osl_to_op_trace P (lce_trace ex)))
+          j (S t);
+    lcsc_complete_clears_current :
+      forall t c j,
+        os_step_label P (lce_trace ex t) (lce_trace ex (S t)) = EvComplete j ->
+        op_current
+          (os_to_op_state (osl_to_os_projection P) (lce_trace ex (S t)))
+          c <> Some j;
+    lcsc_complete_clears_runnable :
+      forall t j,
+        os_step_label P (lce_trace ex t) (lce_trace ex (S t)) = EvComplete j ->
+        ~ In j
+             (op_runnable
+                (os_to_op_state (osl_to_os_projection P) (lce_trace ex (S t))));
+    lcsc_complete_clears_dispatch_target :
+      forall t c j,
+        c < m ->
+        os_step_label P (lce_trace ex t) (lce_trace ex (S t)) = EvComplete j ->
+        op_dispatch_target
+          (os_to_op_state (osl_to_os_projection P) (lce_trace ex (S t)))
+          c <> Some j;
+  }.
+
+Arguments lcsc_wakeup_released
+  {CState P jobs m ex} _ _ _ _.
+Arguments lcsc_wakeup_visible
+  {CState P jobs m ex} _ _ _ _.
+Arguments lcsc_request_sets_need_resched
+  {CState P jobs m ex} _ _ _ _ _.
+Arguments lcsc_handle_sets_need_resched
+  {CState P jobs m ex} _ _ _ _ _.
+Arguments lcsc_choose_sets_dispatch_target
+  {CState P jobs m ex} _ _ _ _ _ _.
+Arguments lcsc_choose_from_runnable
+  {CState P jobs m ex} _ _ _ _ _ _.
+Arguments lcsc_dispatch_sets_current
+  {CState P jobs m ex} _ _ _ _ _ _.
+Arguments lcsc_dispatch_clears_dispatch_target
+  {CState P jobs m ex} _ _ _ _ _ _.
+Arguments lcsc_dispatch_clears_need_resched
+  {CState P jobs m ex} _ _ _ _ _ _.
+Arguments lcsc_dispatch_removes_from_runnable
+  {CState P jobs m ex} _ _ _ _ _ _.
+Arguments lcsc_preempt_sets_current
+  {CState P jobs m ex} _ _ _ _ _ _ _.
+Arguments lcsc_preempt_requeues_old
+  {CState P jobs m ex} _ _ _ _ _ _ _.
+Arguments lcsc_preempt_removes_new_from_runnable
+  {CState P jobs m ex} _ _ _ _ _ _ _.
+Arguments lcsc_preempt_clears_dispatch_target
+  {CState P jobs m ex} _ _ _ _ _ _ _.
+Arguments lcsc_preempt_clears_need_resched
+  {CState P jobs m ex} _ _ _ _ _ _ _.
+Arguments lcsc_complete_sets_completed
+  {CState P jobs m ex} _ _ _ _.
+Arguments lcsc_complete_clears_current
+  {CState P jobs m ex} _ _ _ _ _.
+Arguments lcsc_complete_clears_runnable
+  {CState P jobs m ex} _ _ _ _.
+Arguments lcsc_complete_clears_dispatch_target
+  {CState P jobs m ex} _ _ _ _ _.
+
+Lemma local_labeled_concrete_projection_sound_to_causality_contract :
+  forall CState (P : OSLabeledProjection CState) jobs m
+         (ex : labeled_concrete_execution P m),
+    local_labeled_concrete_projection_sound jobs m ex ->
+    labeled_concrete_scheduling_causality_contract jobs m ex.
+Proof.
+  intros CState P jobs m ex Hlocal.
+  constructor.
+  - intros t j Hwakeup.
+    exact (llcps_wakeup_release Hlocal t j Hwakeup).
+  - intros t j Hwakeup.
+    pose proof (lce_stepwise ex t) as Hstep.
+    rewrite Hwakeup in Hstep.
+    inversion Hstep; subst; clear Hstep.
+    simpl. left. reflexivity.
+  - intros t c Hlt Hreq.
+    exact (llcps_request_sets_need_resched Hlocal t c Hlt Hreq).
+  - intros t c Hlt Hhandle.
+    exact (llcps_handle_sets_need_resched Hlocal t c Hlt Hhandle).
+  - intros t c j Hlt Hchoose.
+    exact (llcps_choose_sets_dispatch_target Hlocal t c j Hlt Hchoose).
+  - intros t c j Hlt Hchoose.
+    exact (llcps_choose_from_runnable Hlocal t c j Hlt Hchoose).
+  - intros t c j Hlt Hdispatch.
+    pose proof (lce_stepwise ex t) as Hstep.
+    rewrite Hdispatch in Hstep.
+    inversion Hstep; subst; clear Hstep.
+    unfold dispatch_on_cpu. simpl.
+    rewrite Nat.eqb_refl.
+    reflexivity.
+  - intros t c j Hlt Hdispatch.
+    pose proof (lce_stepwise ex t) as Hstep.
+    rewrite Hdispatch in Hstep.
+    inversion Hstep; subst; clear Hstep.
+    unfold dispatch_on_cpu. simpl.
+    rewrite Nat.eqb_refl.
+    reflexivity.
+  - intros t c j Hlt Hdispatch.
+    pose proof (lce_stepwise ex t) as Hstep.
+    rewrite Hdispatch in Hstep.
+    inversion Hstep; subst; clear Hstep.
+    unfold dispatch_on_cpu. simpl.
+    rewrite Nat.eqb_refl.
+    reflexivity.
+  - intros t c j Hlt Hdispatch.
+    pose proof (lce_stepwise ex t) as Hstep.
+    rewrite Hdispatch in Hstep.
+    inversion Hstep; subst; clear Hstep.
+    unfold dispatch_on_cpu. simpl.
+    apply remove_job_not_in.
+  - intros t c old new Hlt Hpreempt.
+    pose proof (lce_stepwise ex t) as Hstep.
+    rewrite Hpreempt in Hstep.
+    inversion Hstep; subst; clear Hstep.
+    unfold preempt_on_cpu. simpl.
+    rewrite Nat.eqb_refl.
+    reflexivity.
+  - intros t c old new Hlt Hpreempt.
+    pose proof (lce_stepwise ex t) as Hstep.
+    rewrite Hpreempt in Hstep.
+    inversion Hstep; subst; clear Hstep.
+    unfold preempt_on_cpu. simpl.
+    left. reflexivity.
+  - intros t c old new Hlt Hpreempt.
+    pose proof (lce_stepwise ex t) as Hstep.
+    rewrite Hpreempt in Hstep.
+    inversion Hstep; subst; clear Hstep.
+    unfold preempt_on_cpu. simpl.
+    intros [Heq | Hin].
+    + contradiction.
+    + eapply remove_job_not_in; eauto.
+  - intros t c old new Hlt Hpreempt.
+    pose proof (lce_stepwise ex t) as Hstep.
+    rewrite Hpreempt in Hstep.
+    inversion Hstep; subst; clear Hstep.
+    unfold preempt_on_cpu. simpl.
+    rewrite Nat.eqb_refl.
+    reflexivity.
+  - intros t c old new Hlt Hpreempt.
+    pose proof (lce_stepwise ex t) as Hstep.
+    rewrite Hpreempt in Hstep.
+    inversion Hstep; subst; clear Hstep.
+    unfold preempt_on_cpu. simpl.
+    rewrite Nat.eqb_refl.
+    reflexivity.
+  - intros t j Hcomplete.
+    exact (llcps_complete_sets_completed Hlocal t j Hcomplete).
+  - intros t c j Hcomplete Hcur.
+    pose proof (lce_stepwise ex t) as Hstep.
+    rewrite Hcomplete in Hstep.
+    inversion Hstep; subst; clear Hstep.
+    rewrite <- H1 in Hcur.
+    unfold clear_current_and_request in Hcur. simpl in Hcur.
+    destruct (op_current
+                (os_to_op_state (osl_to_os_projection P) (lce_trace ex t)) c)
+      as [j'|] eqn:Hcur_prev.
+    + destruct (Nat.eqb_spec j' j); congruence.
+    + inversion Hcur.
+  - intros t j Hcomplete.
+    pose proof (lce_stepwise ex t) as Hstep.
+    rewrite Hcomplete in Hstep.
+    inversion Hstep; subst; clear Hstep.
+    unfold clear_current_and_request. simpl.
+    apply remove_job_not_in.
+  - intros t c j Hlt Hcomplete Htarget.
+    pose proof (lce_stepwise ex t) as Hstep.
+    pose proof (lce_struct_inv ex t) as Hinv.
+    rewrite Hcomplete in Hstep.
+    inversion Hstep; subst; clear Hstep.
+    destruct H2 as [c_run Hrun].
+    rewrite <- H1 in Htarget.
+    unfold clear_current_and_request in Htarget. simpl in Htarget.
+    eapply
+      (op_running_job_not_dispatch_pending_in_range
+         m
+         (os_to_op_state (osl_to_os_projection P) (lce_trace ex t))
+         c_run j c); eauto.
+Qed.
+
+Definition os_local_scheduling_causality_contract
+    {CState : Type}
+    {P : OSLabeledProjection CState}
+    {jobs : JobId -> Job}
+    {adm : admissible_cpu}
+    {m : nat}
+    (C : os_local_multicore_adapter_contract P jobs adm m) : Prop :=
+  labeled_concrete_scheduling_causality_contract jobs m (olac_execution C).
+
+Lemma os_local_multicore_adapter_contract_to_causality_contract :
+  forall CState (P : OSLabeledProjection CState) jobs adm m
+         (C : os_local_multicore_adapter_contract P jobs adm m),
+    os_local_scheduling_causality_contract C.
+Proof.
+  intros CState P jobs adm m C.
+  unfold os_local_scheduling_causality_contract.
+  apply local_labeled_concrete_projection_sound_to_causality_contract.
+  exact (llcmps_projection_sound (olac_sound C)).
+Qed.
